Logic/Modal/Normal/Soundness.lean
@@ -8,18 +8,12 @@ open Formula FrameConsequence
 
 variable (α β : Type u) [Inhabited β]
 
-/-
-  TODO: より一般にこの形で証明できる事実ではないだろうか？
-  [LogicK.Hilbert Bew] (Γ : Set (Formula α)) (hΓ : Γ = ∅) (p : Formula α) (f : Frame β) (d : Bew Γ p) : (Γ ⊨ᴹᶠ[f] p)
--/
 lemma Logic.Hilbert.sounds
-  (Λ : Logic (Formula α)) [hΛ : LogicDefines β α Λ]
-  (p : Formula α)
-  (f : Frame β) (hf : LogicDefines.definability Λ f.rel)
+  (Λ : Logic (Formula α))
+  (f : Frame β) (hf : f ∈ (FrameClass β α Λ))
+  {p : Formula α}
   (d : ⊢ᴹ(Λ) p) : (⊧ᴹᶠ[f] p) := by
   induction d <;> try {simp_all [Satisfies];}
-  case maxm p ih =>
-    exact (hΛ.defines f).mp hf p ih;
   case disj₃ p q r =>
     simp only [Frames, Models, Satisfies.imp_def];
     intro V w hpr hqr hpq;
@@ -27,44 +21,28 @@ lemma Logic.Hilbert.sounds
     cases hpq with
     | inl hp => exact hpr hp;
     | inr hq => exact hqr hq;
-  /-
-  case necessitation p dp ih =>
-    simp only [FrameConsequence, Satisfies.box_def];
-    intro V w hΓ w' rww';
-    apply ih V w';
-    intro q hq;
-    exact hw rww' (hΓ q hq);
-  -/
 
 lemma Logic.Hilbert.consistent
-  (Λ : Logic (Formula α)) [hΛ : LogicDefines β α Λ]
+  (Λ : Logic (Formula α))
+  (hf : ∃ f, f ∈ (FrameClass β α Λ))
   : (⊬ᴹ(Λ)! (⊥ : Formula α)) := by
   by_contra hC; simp at hC;
   suffices h : ∃ (f : Frame β), ⊧ᴹᶠ[f] (⊥ : Formula α) by
     let ⟨f, hf⟩ := h;
     exact Frames.bot_def hf;
-  have ⟨tf, htf⟩ := hΛ.trivial_frame;
-  existsi tf; exact Logic.Hilbert.sounds _ _ Λ ⊥ tf htf hC.some;
+  have ⟨tf, htf⟩ := hf;
+  existsi tf;
+  exact Logic.Hilbert.sounds _ _ Λ tf htf hC.some;
 
 variable {α β : Type u} [Inhabited β] {p : Formula α} (f : Frame β)
 
-lemma LogicK.Hilbert.sounds' (hf : (@LogicK.defines β α).definability f.rel)
-  : (⊢ᴹ(𝐊) p) → (⊧ᴹᶠ[f] p) := by
-  exact Logic.Hilbert.sounds _ _ 𝐊 p f hf;
+theorem LogicK.Hilbert.sounds : (⊢ᴹ(𝐊) p) → (⊧ᴹᶠ[f] p) := Logic.Hilbert.sounds _ _ 𝐊 f (def_FrameClass f)
+theorem LogicK.Hilbert.consistency : ⊬ᴹ(𝐊)! (⊥ : Formula α) := Logic.Hilbert.consistent α β 𝐊 (by existsi ((λ _ _ => True)); aesop;)
 
-/--
-  Logic `𝐊` does not require nothing about frames relation.
--/
-theorem LogicK.Hilbert.sounds
-  : (⊢ᴹ(𝐊) p) → (⊧ᴹᶠ[f] p) := by
-  exact LogicK.Hilbert.sounds' _ (by simp)
+theorem LogicKD.Hilbert.sounds (hf : Serial f) (h : ⊢ᴹ(𝐊𝐃) p) : (⊧ᴹᶠ[f] p) := Logic.Hilbert.sounds _ _ 𝐊𝐃 f ((def_FrameClass f).mp hf) h
+theorem LogicKD.Hilbert.consistency : ⊬ᴹ(𝐊𝐃)! (⊥ : Formula α) := Logic.Hilbert.consistent α β 𝐊𝐃 (by existsi ((λ _ _ => True)); aesop;)
 
-theorem LogicK.Hilbert.consistency : ⊬ᴹ(𝐊)! (⊥ : Formula α) := Logic.Hilbert.consistent α β 𝐊
-
-theorem LogicKD.Hilbert.sounds {p : Formula α} (f : Frame β) (hf : (@LogicKD.defines β α).definability f.rel)
-  (h : ⊢ᴹ(𝐊𝐃) p) : (⊧ᴹᶠ[f] p) := by
-  exact Logic.Hilbert.sounds _ _ 𝐊𝐃 p f hf h;
-
-theorem LogicKD.Hilbert.consistency : ⊬ᴹ(𝐊𝐃)! (⊥ : Formula α) := Logic.Hilbert.consistent α β 𝐊𝐃
+-- theorem LogicS4.Hilbert.sounds (hf : Reflexive f ∧ Transitive f) (h : ⊢ᴹ(𝐒𝟒) p) : (⊧ᴹᶠ[f] p) := Logic.Hilbert.sounds _ _ 𝐒𝟒 f ((def_FrameClass f).mp hf) h
+-- theorem LogicS4.Hilbert.consistency : ⊬ᴹ(𝐒𝟒)! (⊥ : Formula α) := Logic.Hilbert.consistent α β 𝐒𝟒 (by existsi ((λ _ _ => True)); aesop;)
 
 end LO.Modal.Normal
